WIP: InstSeq.EqnInv

EffectSSA/ProofSketch/EqnInv.lean
@@ -8,22 +8,12 @@ public section
 
 variable [SSA ι σ ν]
 
-namespace Inst
-
-/-!
-## SSA WellFormedness
--/
-
-/--
-An individual instruction is well-formed, when it doesn't use its own result
-as an argument.
--/
-def WellFormed (i : Inst ι) :=
-  ∀ x ∈ i.args, x ∉ i.results
-
 /-!
 ## Main Definitions
 -/
+@[expose] section Defs
+
+namespace Inst
 
 def EqnInv (i : Inst ι) (ρ : SEnv ι) : Prop :=
   ∀ x ∈ i.results,
@@ -37,12 +27,86 @@ structure WellBehaved (i : Inst ι) where
       → EqnInv i ρ → EqnInv i (⟦j⟧ ρ)
   idempotent: ∀ ρ, EqnInv i (⟦i⟧ ρ)
 
+end Inst
+
+/--
+TODO: the proof ought to work also with a definition of EqnInv/WellBehaved for
+InstSeq that is an analogue of the above for the whole sequence's semantics.
+That would be slightly more general, as it allows for a block to be well-behaved
+as a whole, even if not each instruction is well-behaved indivually.
+For now, though, the simple definition below is good enough.
+-/
+
+abbrev InstSeq.EqnInv (is : InstSeq ι) (ρ : SEnv ι) : Prop :=
+  ∀ i ∈ is, i.EqnInv ρ
+
+abbrev InstSeq.WellBehaved (is : InstSeq ι) : Prop :=
+  ∀ i ∈ is, i.WellBehaved
+
+end Defs
+
+/-!
+## Invariance Lemmas
+-/
+section Invariance
+variable {C : MultiContext ι n} {P : Pattern ι n} {is js : InstSeq ι} {j : Inst ι} {ρ : SEnv ι}
+
+/-! ### InstSeq -/
+namespace InstSeq
+
+@[simp, grind .] theorem eqnInv_nil : EqnInv ([] : InstSeq ι) ρ := by grind
+@[simp] theorem eqnInv_cons : (i ;> is).EqnInv ρ ↔ i.EqnInv ρ ∧ is.EqnInv ρ := by grind
+
+theorem eqnInv_denote_inst (h : is.WellBehaved)
+    (hj : ∀ x ∈ j.results, x ∉ is.args ∧ x ∉ is.results) :
+    is.EqnInv ρ → is.EqnInv (⟦j⟧ ρ) := by
+  sorry
+
+theorem eqnInv_denote_other (h : is.WellBehaved) (hwf : js.WellFormed Γ)
+    (hres : is.results ⊆ Γ) (hargs : is.args ⊆ Γ) :
+    is.EqnInv ρ → is.EqnInv (⟦js⟧ ρ) := by
+  intro hρ
+  induction js generalizing ρ
+  · grind
+  case cons _ _ ih =>
+    simp only [denote_cons]
+    apply ih
+    · sorry
+    apply eqnInv_denote_inst
+    · assumption
+    · sorry
+    · assumption
+
+theorem eqnInv_denote_self (h : is.WellBehaved) (hwf : is.NoShadowing) :
+    is.EqnInv (⟦is⟧ ρ) := by
+  stop
+  intro i' hi'
+  induction is generalizing ρ
+  · contradiction
+  case cons i is ih =>
+    simp only [denote_cons, eqnInv_cons]
+    and_intros
+    · apply eqnInv_denote_other
+    · apply ih <;> grind
+
+end InstSeq
+
+/-! ### Context Plugging-/
+namespace MultiContext
+
+theorem foo :
+
+end MultiContext
+
+end Invariance
+
 /-!
 ## Locally Pure
 Justify the well-behavedness predicate by showing that all so-called
 "locally pure" instructions are well-behaved.
 -/
 section LocallyPure
+open Inst
 
 /--
 An instruction is *locally pure*, when it's effect on local registers,
@@ -50,7 +114,7 @@ is determined purely from the local registers.
 
 To wit: such an instruction is free to modify the *global state* in any way.
 -/
-@[expose] def LocallyPure (i : Inst ι) : Prop :=
+@[expose] def Inst.LocallyPure (i : Inst ι) : Prop :=
   ∀ ρ η, ρ.locals = η.locals →
     (⟦i⟧ ρ).locals = (⟦i⟧ η).locals
 
@@ -62,6 +126,13 @@ theorem locallyPure_imp (i : Inst ι) :
   calc (⟦i⟧ ρ).locals x
     _ = (⟦i⟧ η').locals x := by have := denote_eq_of_args i ρ η'; grind only
     _ = (⟦i⟧ η).locals x := by grind [LocallyPure]
+
+/--
+An individual instruction is well-formed, when it doesn't use its own result
+as an argument.
+-/
+@[expose] def Inst.WellFormed (i : Inst ι) :=
+  ∀ x ∈ i.args, x ∉ i.results
 
 /--
 Every purely determined instruction, is well-behaved.
